add a requirement that R is total to cequiv

cava/Cava/Semantics/Equivalence.v
@@ -23,52 +23,108 @@ Require Import Cava.Semantics.Simulation.
 Require Import Cava.Util.List.
 Require Import Cava.Util.Tactics.
 
+(* states that a relation is total *)
+Definition is_total {A B} (R : A -> B -> Prop) : Prop :=
+  (forall a, exists b, R a b) /\ (forall b, exists a, R a b).
+
 (* Circuit equivalence relation *)
 Definition cequiv {i o} (c1 c2 : Circuit i o) : Prop :=
   (* there exists some relation between the circuit states... *)
   exists (R : value (circuit_state c1) -> value (circuit_state c2) -> Prop),
-    (* ...and the relation holds on the reset states *)
-    R (reset_state c1) (reset_state c2)
-    (* ...and if the relation holds, stepping each circuit on the same input
-         results in the same output as well as new states on which the relation
-         continues to hold *)
+    (* ...and the relation is total *)
+    is_total R
+    (* ...and the reset states are related *)
+    /\ R (reset_state c1) (reset_state c2)
+    (* ...and if the states are related, stepping each circuit on the same input
+         results in the same output as well as new related states *)
     /\ (forall s1 s2 input,
           R s1 s2 ->
           snd (step c1 s1 input) = snd (step c2 s2 input)
           /\ R (fst (step c1 s1 input)) (fst (step c2 s2 input))).
 
+(* TODO: move? *)
+Lemma ex_split_pair {A B} (P : A * B -> Prop) :
+  (exists a b, P (a,b)) -> (exists ab, P ab).
+Proof. intros. logical_simplify. eexists; eauto. Qed.
+
+(* TODO: move? *)
+Ltac eexists_destruct :=
+  repeat lazymatch goal with
+         | |- exists _ : (_ * _)%type, _ => apply ex_split_pair
+         | |- exists _ : unit, _ => exists tt
+         | |- exists _, _ => eexists
+         end.
+
+(* solve is_total side conditions *)
+Ltac solve_is_total :=
+  cbv [is_total] in *; intros; logical_simplify;
+  ssplit; intros;
+  destruct_products; cbn [fst snd] in *;
+  logical_simplify;
+  repeat lazymatch goal with
+         | H : (forall x : ?T, exists _, _), x :?T |- _ =>
+           specialize (H x); logical_simplify
+         end;
+  (* the eexists/eauto might produce shelved existential variables if some
+     pieces of state appear in one circuit's state but not the other's; try to plug
+     in default values for the unused variables, and fail if we can't *)
+  unshelve (eexists_destruct; cbn[fst snd]; (solve [ eauto ]));
+  lazymatch goal with
+  | |- unit => exact tt
+  | |- value _ => exact defaultValue
+  | |- ?x => fail "could not infer default value for unused state value with type" x
+  end.
+
+(* find the hypothesis saying circuit state equivalence is preserved over
+   [step], and specialize it to the current arguments *)
+Local Ltac use_preserved :=
+  lazymatch goal with
+  | H : (forall _ _ _, ?R _ _ -> _ /\ _), HR : ?R ?s1 ?s2
+    |- context [step _ ?s1 ?i] =>
+    let H1 := fresh in
+    let H2 := fresh in
+    specialize (H s1 s2 i HR); destruct H as [H1 H2];
+    rewrite ?H1, ?H2
+end.
+
 (* cequiv is transitive *)
 Global Instance Transitive_cequiv {i o} : Transitive (@cequiv i o) | 10.
 Proof.
-  intros x y z [Rxy [? Hxy]] [Ryz [? Hyz]]. logical_simplify.
-  exists (fun (st1 : value (circuit_state x)) (st2 : value (circuit_state z)) =>
-       exists st3 : value (circuit_state y), Rxy st1 st3 /\ Ryz st3 st2).
-  ssplit; [ exists (reset_state y); tauto | ].
-  intros; logical_simplify.
-  specialize (Hxy _ _ ltac:(eassumption) ltac:(eassumption)).
-  specialize (Hyz _ _ ltac:(eassumption) ltac:(eassumption)).
-  logical_simplify. ssplit; [ congruence | ]. eauto.
+  intros x y z [Rxy [? [? Hxy]]] [Ryz [? [? Hyz]]].
+  logical_simplify. exists (fun x z => exists y, Rxy x y /\ Ryz y z).
+  ssplit; [ solve_is_total | solve [eauto] | ].
+  intros; logical_simplify; subst.
+  repeat use_preserved. ssplit; eauto.
 Qed.
 
 (* cequiv is reflexive *)
 Global Instance Reflexive_cequiv {i o} : Reflexive (@cequiv i o) | 10.
 Proof.
-  repeat intro. exists eq. ssplit; [ reflexivity | ].
+  repeat intro. exists eq. ssplit; [ solve_is_total | reflexivity | ].
   intros; subst. ssplit; reflexivity.
 Qed.
 
 (* cequiv is symmetric *)
 Global Instance Symmetric_cequiv {i o} : Symmetric (@cequiv i o) | 10.
 Proof.
-  intros x y [R [? HR]]. logical_simplify.
-  exists (fun st1 st2 => R st2 st1). ssplit; [ assumption | ].
-  intros. specialize (HR _ _ ltac:(eassumption) ltac:(eassumption)).
-  logical_simplify. eauto.
+  intros x y [Rxy [? [? Hxy]]]. logical_simplify. exists (fun y x => Rxy x y).
+  ssplit; [ solve_is_total | solve [eauto] | ].
+  intros; logical_simplify; subst.
+  repeat use_preserved. ssplit; eauto.
 Qed.
 
 (* cequiv is an equivalence relation *)
 Global Instance Equivalence_cequiv {i o} : Equivalence (@cequiv i o) | 10.
 Proof. constructor; typeclasses eauto. Qed.
+
+(* Try to solve [Proper] goals with cequiv *)
+Local Ltac proper_hammer :=
+  cbn [reset_state circuit_state fst snd value] in *; fold @value combType in *;
+  ssplit; intros; destruct_products; cbn [fst snd] in *;
+    [ solve_is_total | solve [eauto] .. | ];
+  cbn [circuit_state step fst snd]; intros; logical_simplify; subst;
+  cbn [value]; fold @value combType in *;
+  repeat use_preserved; ssplit; try congruence.
 
 (* equivalent circuits produce the same output on the same input *)
 Lemma simulate_cequiv {i o} (c1 c2 : Circuit i o) :
@@ -79,15 +135,8 @@ Proof.
     with (I:=fun st1 st2 acc1 acc2 =>
                R st1 st2 /\ acc1 = acc2).
   { ssplit; eauto. }
-  { intros; logical_simplify; subst.
-    lazymatch goal with
-    | H : forall _ _ _, R _ _ -> _ /\ _, HR : R _ _ |- context [step _ _ ?i] =>
-    let H1 := fresh in
-    let H2 := fresh in
-    specialize (H _ _ i HR); destruct H as [H1 H2];
-      rewrite ?H1, ?H2
-    end.
-    ssplit; eauto. }
+  { intros; logical_simplify; subst. use_preserved.
+    ssplit; congruence. }
   { intros; logical_simplify; subst. reflexivity. }
 Qed.
 
@@ -102,67 +151,28 @@ Global Instance Proper_LoopInitCE {i s o} :
 Proof.
   repeat intro; subst.
   lazymatch goal with H : cequiv _ _ |- _ => destruct H as [R ?] end.
-  logical_simplify.
-  exists (fun st1 st2 => R (fst st1) (fst st2) /\ snd st1 = snd st2).
-  cbn [reset_state circuit_state fst snd] in *.
-  ssplit; [ solve [auto] .. | ]. intros; logical_simplify.
-  cbn [value] in *. destruct_products; cbn [fst snd] in *; subst.
-  cbn [step]. simpl_ident.
-  repeat destruct_pair_let; cbn [fst snd]. cbn [value]. fold @value combType.
-  lazymatch goal with
-  | H : forall _ _ _, R _ _ -> _ /\ _, HR : R _ _ |- context [step _ _ ?i] =>
-  let H1 := fresh in
-  let H2 := fresh in
-  specialize (H _ _ i HR); destruct H as [H1 H2];
-    rewrite ?H1, ?H2
-  end.
-  ssplit; eauto.
+  exists (fun s1 s2 => R (fst s1) (fst s2) /\ snd s1 = snd s2).
+  proper_hammer.
 Qed.
 
 (* cequiv c1 c3 -> cequiv c2 c4 -> cequiv (c1 >==> c2) (c3 >==> c4) *)
 Global Instance Proper_Compose {i t o} :
   Proper (cequiv ==> cequiv ==> cequiv) (@Compose _ _ i t o).
 Proof.
-  intros a b [Rab [? Hab]].
-  intros c d [Rcd [? Hcd]].
-  exists (fun st1 st2 => Rab (fst st1) (fst st2) /\ Rcd (snd st1) (snd st2)).
-  ssplit; [ assumption .. | ].
-  cbn [circuit_state step]. intros; logical_simplify.
-  pose proof (fun i => proj1 (Hab _ _ i ltac:(eassumption))) as Hab1.
-  pose proof (fun i => proj2 (Hab _ _ i ltac:(eassumption))) as Hab2.
-  pose proof (fun i => proj1 (Hcd _ _ i ltac:(eassumption))) as Hcd1.
-  pose proof (fun i => proj2 (Hcd _ _ i ltac:(eassumption))) as Hcd2.
-  clear Hab Hcd. logical_simplify.
-  repeat (destruct_pair_let; cbn [fst snd]).
-  rewrite ?Hab1, ?Hcd1.
-  ssplit; eauto; [ apply Hab2 | apply Hcd2 ].
+  intros a b [Rab ?] c d [Rcd ?].
+  exists (fun ac bd => Rab (fst ac) (fst bd) /\ Rcd (snd ac) (snd bd)).
+  proper_hammer.
 Qed.
 
 (* cequiv c1 c2 -> cequiv (First c1) (First c2) *)
 Global Instance Proper_First {i o t} :
   Proper (cequiv ==> cequiv) (@First _ _ i o t).
-Proof.
-  intros x y [Rxy [? Hxy]].
-  exists Rxy; ssplit; [ assumption | ].
-  cbn [circuit_state step]. intros; logical_simplify.
-  pose proof (fun i => proj1 (Hxy _ _ i ltac:(eassumption))) as Hxy1.
-  pose proof (fun i => proj2 (Hxy _ _ i ltac:(eassumption))) as Hxy2.
-  clear Hxy. logical_simplify. repeat (destruct_pair_let; cbn [fst snd]).
-  rewrite Hxy1. ssplit; eauto.
-Qed.
+Proof. intros x y [R ?]. exists R. proper_hammer. Qed.
 
 (* cequiv c1 c2 -> cequiv (Second c1) (Second c2) *)
 Global Instance Proper_Second {i o t} :
   Proper (cequiv ==> cequiv) (@Second _ _ i o t).
-Proof.
-  intros x y [Rxy [? Hxy]].
-  exists Rxy; ssplit; [ assumption | ].
-  cbn [circuit_state step]. intros; logical_simplify.
-  pose proof (fun i => proj1 (Hxy _ _ i ltac:(eassumption))) as Hxy1.
-  pose proof (fun i => proj2 (Hxy _ _ i ltac:(eassumption))) as Hxy2.
-  clear Hxy. logical_simplify. repeat (destruct_pair_let; cbn [fst snd]).
-  rewrite Hxy1. ssplit; eauto.
-Qed.
+Proof. intros x y [R ?]. exists R. proper_hammer. Qed.
 
 (* r1 = r2 -> cequiv c1 c2 -> cequiv (LoopInit r1 c1) (LoopInit r2 c2) *)
 Global Instance Proper_LoopInit {i s o} :
